lunarlander_sl/Velocity.thy
@@ -1,0 +1,302 @@
+theory Velocity
+  imports ContinuousInv
+begin
+
+
+subsection \<open>Test of velocity control\<close>
+
+definition V :: char where "V = CHR ''v''"
+definition A :: char where "A = CHR ''a''"
+definition T :: char where "T = CHR ''t''"
+
+lemma [simp]: "V \<noteq> A" "A \<noteq> V" "V \<noteq> T" "T \<noteq> V" "A \<noteq> T" "T \<noteq> A"
+  by (auto simp add: V_def A_def T_def)
+
+definition plant :: proc where
+  "plant = Rep (T ::= (\<lambda>_. 0);
+                Cont (ODE ((\<lambda>_ _. 0)(V := (\<lambda>s. s A), T := (\<lambda>_. 1)))) (\<lambda>s. s T < 1);
+                Cm (''p2c''[!](\<lambda>s. s V));
+                Cm (''c2p''[?]A))"
+
+definition control :: proc where
+  "control = Rep (Cm (''p2c''[?]V);
+                  Cm (''c2p''[!](\<lambda>s. if s V < 10 then 1 else -1)))"
+
+definition system :: pproc where
+  "system = Parallel (Single plant) {''p2c'', ''c2p''} (Single control)"
+
+lemma plant_ODE:
+  "\<Turnstile> {\<lambda>s tr. s = (\<lambda>_. 0)(V := v0, A := a0, T := 0) \<and> P tr}
+        Cont (ODE ((\<lambda>_ _. 0)(V := (\<lambda>s. s A), T := (\<lambda>_. 1)))) (\<lambda>s. s T < 1)
+      {\<lambda>s tr. s = (\<lambda>_. 0)(V := v0 + a0 * 1, A := a0, T := 1) \<and>
+              (P @\<^sub>t WaitS\<^sub>t 1 (\<lambda>t. (\<lambda>_. 0)(V := v0 + a0 * t, A := a0, T := t)) ({}, {})) tr}"
+proof -
+  have 1: "ODEsol (ODE ((\<lambda>_ _. 0)(V := (\<lambda>s. s A), T := (\<lambda>_. 1))))
+                  (\<lambda>t. (\<lambda>_. 0)(V := v0 + a0 * t, A := a0, T := t)) 1"
+    unfolding ODEsol_def has_vderiv_on_def
+    apply auto
+    apply (rule has_vector_derivative_projI)
+    apply (auto simp add: state2vec_def A_def V_def T_def)
+     apply (rule has_vector_derivative_eq_rhs)
+      apply (auto intro!: derivative_intros)[1] apply simp
+    subgoal for x i
+      apply (cases "i = CHR ''a''") by auto
+    done
+  have 2: "local_lipschitz {- (1::real)<..} UNIV (\<lambda>t v. ODE2Vec (ODE ((\<lambda>_ _. 0)(V := \<lambda>s. s A, T := \<lambda>_. 1))) (vec2state v))"
+  proof -
+    show ?thesis
+      unfolding state2vec_def vec2state_def fun_upd_def
+      apply (rule c1_implies_local_lipschitz[where f'="(\<lambda>(t,v). Blinfun(\<lambda>(v::vec) . \<chi> x. if x = V then (v$A) else if x = T then 0 else 0))"])
+         apply auto
+      subgoal for t x
+        apply (subst bounded_linear_Blinfun_apply)
+        subgoal
+          apply (rule bounded_linearI')
+          by (auto simp add: vec_lambda_unique[symmetric])
+        unfolding has_derivative_def
+        apply auto
+          apply (rule bounded_linearI')
+        apply (auto simp add: vec_lambda_unique[symmetric])
+        apply (rule vec_tendstoI)
+        by (auto simp add: state2vec_def)
+      done
+  qed
+  show ?thesis
+    apply (rule Valid_ode_unique_solution'[OF _ 1 _ _ _ 2])
+    by auto
+qed
+
+fun plant_inv :: "real \<times> real \<times> real \<Rightarrow> real list \<Rightarrow> tassn" where
+  "plant_inv (v0, a0, t0) [] = emp\<^sub>t"
+| "plant_inv (v0, a0, t0) (a # as) =
+     WaitS\<^sub>t 1 (\<lambda>t. (\<lambda>_. 0)(V := v0 + a0 * t, A := a0, T := t)) ({}, {}) @\<^sub>t
+     Out\<^sub>t ((\<lambda>_. 0)(V := v0 + a0, A := a0, T := 1)) ''p2c'' (v0 + a0) @\<^sub>t
+     In\<^sub>t ((\<lambda>_. 0)(V := v0 + a0, A := a0, T := 1)) ''c2p'' a @\<^sub>t
+     plant_inv (v0 + a0, a, 1) as"
+
+fun plant_end_state :: "real \<times> real \<times> real \<Rightarrow> real list \<Rightarrow> state" where
+  "plant_end_state (v0, a0, t0) [] = ((\<lambda>_. 0)(V := v0, A := a0, T := t0))"
+| "plant_end_state (v0, a0, t0) (a # as) =
+   plant_end_state (v0 + a0, a, 1) as"
+
+lemma plant_end_state_rw:
+  "(plant_end_state (v0, a0, t0) as)(T := 0) =
+   (\<lambda>_. 0)(V := plant_end_state (v0, a0, t0) as V,
+           A := plant_end_state (v0, a0, t0) as A,
+           T := 0)"
+  apply (induct as arbitrary: v0 a0 t0) by auto
+
+lemma plant_end_state_snoc:
+  "plant_end_state (v0, a0, t0) (as @ [a]) =
+   (\<lambda>_. 0)(V := plant_end_state (v0, a0, t0) as V + plant_end_state (v0, a0, t0) as A, T := 1, A := a)"
+  apply (induct as arbitrary: v0 a0 t0) by auto
+
+lemma plant_inv_snoc:
+  "plant_inv (v0, a0, t0) (xs @ [a]) =
+  (plant_inv (v0, a0, t0) xs @\<^sub>t
+   WaitS\<^sub>t 1 (\<lambda>t. (\<lambda>_. 0) (V := plant_end_state (v0, a0, t0) xs V + plant_end_state (v0, a0, t0) xs A * t,
+                          A := plant_end_state (v0, a0, t0) xs A, T := t)) ({}, {})) @\<^sub>t
+   Out\<^sub>t ((\<lambda>_. 0) (V := plant_end_state (v0, a0, t0) xs V + plant_end_state (v0, a0, t0) xs A,
+                  A := plant_end_state (v0, a0, t0) xs A, T := 1))
+       ''p2c'' (plant_end_state (v0, a0, t0) xs V + plant_end_state (v0, a0, t0) xs A) @\<^sub>t
+   In\<^sub>t ((\<lambda>_. 0) (V := plant_end_state (v0, a0, t0) xs V + plant_end_state (v0, a0, t0) xs A,
+                 A := plant_end_state (v0, a0, t0) xs A, T := 1))
+       ''c2p'' a"
+proof (induct xs arbitrary: v0 a0 t0)
+  case Nil
+  have a: "(\<lambda>_. 0)(V := v0 + a0 * t, A := a0, T := t) =
+        (\<lambda> a. if a = T then t else if a = A then a0 else if a = V then v0 + a0 * t else 0)" for t
+    apply (rule ext) by auto
+  have b: "(\<lambda>_. 0)(V := v0 + a0, A := a0, T := 1) =
+        (\<lambda> a. if a = T then 1 else if a = A then a0 else if a = V then v0 + a0 else 0)"
+    apply (rule ext) by auto
+  show ?case
+    by (auto simp add: a b)
+next
+  case (Cons a as)
+  show ?case
+    by (auto simp add: Cons join_assoc)
+qed
+
+lemma plant_prop:
+  "\<Turnstile> {\<lambda>s tr. s = (\<lambda>_. 0)(V := v0, A := a0, T := t0) \<and> emp\<^sub>t tr}
+        plant
+      {\<lambda>s tr. \<exists>as. s = plant_end_state (v0, a0, t0) as \<and>
+                   plant_inv (v0, a0, t0) as tr}"
+  unfolding plant_def
+  apply (rule Valid_weaken_pre)
+   prefer 2 apply (rule Valid_rep)
+  apply (rule Valid_ex_pre)
+  subgoal for xs
+    apply (rule Valid_seq)
+    apply (rule Valid_assign_sp)
+    apply (rule Valid_seq)
+    unfolding plant_end_state_rw
+     apply (rule plant_ODE)
+    apply (rule Valid_seq)
+     apply (rule Valid_send_sp)
+    apply (rule Valid_strengthen_post)
+     prefer 2 apply (rule Valid_receive_sp)
+    apply (auto simp add: entails_def)
+    subgoal for tr a
+      apply (rule exI[where x="xs @ [a]"])
+      by (auto simp add: plant_end_state_snoc plant_inv_snoc join_assoc)
+    done
+  apply (auto simp add: entails_def)
+  apply (rule exI[where x="[]"])
+  by auto
+
+fun control_inv :: "real \<Rightarrow> real list \<Rightarrow> tassn" where
+  "control_inv v0 [] = emp\<^sub>t"
+| "control_inv v0 (v # vs) =
+   In\<^sub>t ((\<lambda>_. 0)(V := v0)) ''p2c'' v @\<^sub>t
+   Out\<^sub>t ((\<lambda>_. 0)(V := v)) ''c2p'' (if v < 10 then 1 else -1) @\<^sub>t
+   control_inv v vs"
+
+fun control_end_state :: "real \<Rightarrow> real list \<Rightarrow> state" where
+  "control_end_state v0 [] = ((\<lambda>_. 0)(V := v0))"
+| "control_end_state v0 (v # vs) = control_end_state v vs"
+
+lemma control_end_state_snoc:
+  "control_end_state v0 (vs @ [v]) = (control_end_state v0 vs)(V := v)"
+  apply (induct vs arbitrary: v0) by auto
+
+lemma control_inv_snoc:
+  "control_inv v0 (vs @ [v]) =
+   control_inv v0 vs @\<^sub>t In\<^sub>t (control_end_state v0 vs) ''p2c'' v @\<^sub>t Out\<^sub>t ((control_end_state v0 vs)(V := v)) ''c2p''
+   (if v < 10 then 1 else -1)"
+proof (induct vs arbitrary: v0)
+  case Nil
+  have a: "(\<lambda>_. 0)(V := v0) = (\<lambda>a. if a = V then v0 else 0)"
+    apply (rule ext) by auto
+  have aa: "(\<lambda>_. 0)(V := v) = (\<lambda>a. if a = V then v else if a = V then v0 else 0)"
+    apply (rule ext) by auto
+  show ?case
+    by (auto simp add: a aa)
+next
+  case (Cons a vs)
+  then show ?case
+    by (auto simp add: join_assoc)
+qed
+
+
+lemma control_prop:
+  "\<Turnstile> {\<lambda>s tr. s = (\<lambda>_. 0)(V := v0) \<and> emp\<^sub>t tr}
+        control
+      {\<lambda>s tr. \<exists>vs. s = control_end_state v0 vs \<and>
+                   control_inv v0 vs tr}"
+  unfolding control_def
+  apply (rule Valid_weaken_pre)
+   prefer 2 apply (rule Valid_rep)
+   apply (rule Valid_ex_pre)
+  subgoal for vs
+    apply (rule Valid_seq)
+     apply (rule Valid_receive_sp)
+    apply (rule Valid_ex_pre)
+    subgoal for v
+      apply (rule Valid_strengthen_post)
+       prefer 2 apply (rule Valid_send_sp)
+      apply (auto simp add: entails_def)
+      apply (rule exI[where x="vs @ [v]"])
+       apply (auto simp add: control_end_state_snoc control_inv_snoc join_assoc)
+      apply (rule exI[where x="vs @ [v]"])
+      by (auto simp add: control_end_state_snoc control_inv_snoc join_assoc)
+    done
+  apply (auto simp add: entails_def)
+  apply (rule exI[where x="[]"])
+  by auto
+
+
+fun loop_inv :: "real \<times> real \<Rightarrow> bool" where
+  "loop_inv (v, a) \<longleftrightarrow> (v \<ge> 9 \<and> v \<le> 11 \<and> a = (if v < 10 then 1 else -1))"
+
+declare loop_inv.simps [simp del]
+
+fun system_inv :: "nat \<Rightarrow> tassn" where
+  "system_inv 0 = emp\<^sub>t"
+| "system_inv (Suc n) = (\<exists>\<^sub>tv0 a0 v0'. \<up>(loop_inv (v0, a0)) \<and>\<^sub>t
+     Wait\<^sub>t 1 (\<lambda>t. ParState (State ((\<lambda>_. 0)(V := v0 + a0 * t, A := a0, T := t))) (State ((\<lambda>_. 0)(V := v0')))) ({}, {''p2c''}) @\<^sub>t
+     IO\<^sub>t ''p2c'' (v0 + a0) @\<^sub>t
+     IO\<^sub>t ''c2p'' (if v0 + a0 < 10 then 1 else -1) @\<^sub>t
+     system_inv n)"
+
+lemma combine:
+  "loop_inv (v0, a0) \<Longrightarrow>
+   combine_assn {''p2c'', ''c2p''}
+    (plant_inv (v0, a0, t0) as) (control_inv v0' vs) \<Longrightarrow>\<^sub>t system_inv (length as)"
+proof (induct as arbitrary: v0 a0 t0 v0' vs)
+  case Nil
+  then show ?case
+  proof (cases vs)
+    case Nil
+    then show ?thesis by auto
+  next
+    case (Cons a list)
+    then show ?thesis
+      by (auto simp add: combine_assn_emp_in)
+  qed
+next
+  case (Cons a as)
+  note Cons1 = Cons
+  then show ?case
+  proof (cases vs)
+    case Nil
+    then show ?thesis
+      apply auto
+      apply (rule entails_tassn_trans)
+      apply (rule combine_assn_wait_emp)
+      by (rule false_assn_entails)
+  next
+    case (Cons v vs)
+    show ?thesis
+      apply (auto simp add: Cons split del: if_split)
+      apply (rule entails_tassn_trans)
+      apply (rule combine_assn_wait_in)
+      apply (auto split del: if_split)
+      apply (rule entails_tassn_exI[where x=v0])
+      apply (rule entails_tassn_exI[where x=a0])
+      apply (rule entails_tassn_exI[where x=v0'])
+      apply (rule entails_tassn_conj)
+      subgoal
+        by (auto simp add: pure_assn_def Cons1(2) entails_tassn_def)
+      apply (rule entails_tassn_cancel_left)
+      apply (rule entails_tassn_trans)
+       apply (rule combine_assn_out_in)
+       apply (auto split del: if_split)
+      apply (rule entails_tassn_cancel_left)
+      apply (rule entails_tassn_trans)
+       apply (rule combine_assn_in_out)
+       apply (auto split del: if_split)
+      apply (rule entails_tassn_cancel_left)
+      apply (rule Cons1(1))
+      using Cons1(2) by (auto simp add: loop_inv.simps)
+  qed
+qed
+
+theorem system_prop:
+  assumes "loop_inv (v0, a0)"
+  shows "\<Turnstile>\<^sub>p
+    {pair_assn (\<lambda>s. s = ((\<lambda>_. 0)(V := v0, A := a0, T := t0)))
+               (\<lambda>s. s = ((\<lambda>_. 0)(V := v0')))}
+      system
+    {\<exists>\<^sub>g n. trace_gassn (system_inv n)}"
+  unfolding system_def
+  apply (rule ParValid_conseq')
+  apply (rule ParValid_Parallel')
+  apply (rule plant_prop)
+  apply (rule control_prop)
+   apply (auto simp add: sing_gassn_split sing_gassn_ex)
+  apply (rule sync_gassn_ex_pre_left)
+  apply (rule sync_gassn_ex_pre_right)
+  subgoal for as vs
+    unfolding sync_gassn_state_left sync_gassn_state_right
+    apply (rule entails_ex_gassn)
+    apply (rule exI[where x="length as"])
+    apply (rule and_entails_gassn2[OF sync_gassn_traces])
+    apply (rule and_entails_gassn2[OF entails_trace_gassn])
+    apply (rule combine[OF assms])
+    by (auto simp add: entails_tassn_def entails_gassn_def and_gassn_def)
+  done
+
+
+end
